

# Riemann Sum for

$$f(x) = 3x + 2x^2 \text{ over } [0, 1]$$

$$\Delta x = \frac{1-0}{n} = \frac{1}{n}$$

$$c_k = a + k\Delta x = 0 + k\left(\frac{1}{n}\right) = \frac{k}{n}$$

$$f(c_k) = \frac{3k}{n} + \frac{2k^2}{n^2}$$

$$S_n = \sum_{k=1}^n \left( \frac{3k}{n} + \frac{2k^2}{n^2} \right) \cdot \frac{1}{n}$$

$$S_n = \sum_{k=1}^n \left( \frac{3k}{n^2} + \frac{2k^2}{n^3} \right)$$

$$S_n = \frac{3}{n^2} \sum_{k=1}^n k + \frac{2}{n^3} \sum_{k=1}^n k^2$$

$$S_n = \frac{3}{n^2} \left( \frac{n(n+1)}{2} \right) + \frac{2}{n^3} \left( \frac{n(n+1)(2n+1)}{6} \right)$$

$$S_n = \frac{3(n+1)}{2n} + \frac{(n+1)(2n+1)}{3n^2}$$

$$\text{Area} = \lim_{n \rightarrow \infty} \left( \frac{3(n+1)}{2n} + \frac{(n+1)(2n+1)}{3n^2} \right)$$

$$\lim_{n \rightarrow \infty} = \left( \frac{3}{2} + \frac{3}{n^2} + \frac{2}{3} + \frac{1}{n} + \frac{1}{3n^2} \right)$$

$$\lim_{n \rightarrow \infty} = \left( \frac{3}{2} + 0 + \frac{2}{3} + 0 + 0 \right) \rightarrow$$

$$\lim_{n \rightarrow \infty} = \boxed{\frac{13}{6}}$$

for  $f(x) = x^2 - x^3$  on  $[-1, 0]$

$$\Delta x = \frac{1}{n}$$

$$c_k = -1 + \frac{k}{n}$$

$$f(c_k) = \left(-1 + \frac{k}{n}\right)^2 - \left(-1 + \frac{k}{n}\right)^3$$

$$f(c_k) = 2 - \frac{5k}{n} + \frac{4k^2}{n^2} - \frac{k^3}{n^3}$$

$$S_n = \sum_{k=1}^n \left( 2 - \frac{5k}{n} + \frac{4k^2}{n^2} - \frac{k^3}{n^3} \right) \cdot \frac{1}{n}$$

$$S_n = \sum_{k=1}^n \left( \frac{2}{n} - \frac{5k}{n^2} + \frac{4k^2}{n^3} - \frac{k^3}{n^4} \right)$$

$$S_n = \frac{2}{n} \sum_{k=1}^n 1 - \frac{5}{n^2} \sum_{k=1}^n k + \frac{4}{n^3} \sum_{k=1}^n k^2 - \frac{1}{n^4} \sum_{k=1}^n k^3$$

$$S_n = \frac{2}{n} n - \frac{5}{n^2} \left( \frac{n(n+1)}{2} \right) + \frac{4}{n^3} \left( \frac{n(n+1)(2n+1)}{6} \right) - \frac{1}{n^4} \left( \frac{n^2(n+1)^2}{4} \right)$$

$$\lim_{n \rightarrow \infty} S_n = \left( 2 - \frac{5(n+1)}{2n} + \frac{2(n+1)}{3n^2} + \frac{2(n+1)(2n+1)}{3n^2} - \frac{n^2}{4n^2} \right)$$

$$\text{Area} = 2 - \frac{5}{2} + \frac{4}{3} - \frac{1}{4}$$

$$\text{Area} = \frac{7}{12}$$

for  $\int_1^e \ln(x) dx$

$$\Delta x = \frac{e-1}{n}$$

$$c_k = 1 + k \left( \frac{e-1}{n} \right)$$

$$f(c_k) = \ln \left( 1 + k \frac{e-1}{n} \right)$$

$$S_n = \sum_{k=1}^n \left( \ln \left( 1 + k \frac{e-1}{n} \right) \right) \left( \frac{e-1}{n} \right)$$

$$S_n = \frac{e-1}{n} \sum_{k=1}^n \ln \left( 1 + k \frac{e-1}{n} \right)$$

Definite Integral for  $\lim_{\Delta x \rightarrow 0} \sum f(x) \Delta x$

$$\lim_{\Delta x \rightarrow 0} \sum_{k=1}^n f(c_k) \Delta x = \int_a^b f(x) dx$$

$$\text{Area} = \lim_{n \rightarrow \infty} \sum_{k=1}^n f(c_k) \Delta x$$

$$f(x) = x^2 - x^3 \quad [a, b] = [-1, 0]$$

$$\Delta x = \frac{b-a}{n} = \frac{1}{n}$$

$$c_k = a + k \Delta x = -1 + k \frac{1}{n} = \frac{k}{n} - 1$$

$$f(c_k) = (c_k)^2 - (c_k)^3 \rightarrow f(c_k) = \left( \frac{k}{n} - 1 \right)^2 - \left( \frac{k}{n} - 1 \right)^3$$

$$f(c_k) = \left[ \frac{k^2}{n^2} - \frac{2k}{n} + 1 \right] - \left[ \frac{k^3}{n^3} - \frac{3k^2}{n^2} + \frac{3k}{n} - 1 \right]$$

$$f(k) = -\frac{1}{n^3}k^3 + \frac{4}{n^2}k^2 - \frac{5}{n}k + 2$$

$$\sum_{k=1}^n \left( -\frac{1}{n^3}k^3 + \frac{4}{n^2}k^2 - \frac{5}{n}k + 2 \right) \cdot \frac{1}{n}$$

$$\sum_{k=1}^n \left( -\frac{1}{n^4}k^3 + \frac{4}{n^3}k^2 - \frac{5}{n^2}k + \frac{2}{n} \right)$$

$$-\frac{1}{n^4} \sum_{k=1}^n k^3 + \frac{4}{n^3} \sum_{k=1}^n k^2 - \frac{5}{n^2} \sum_{k=1}^n k + \sum_{k=1}^n \frac{2}{n}$$

$$-\frac{1}{n^4} \left[ \frac{n^2(n+1)^2}{4} \right] + \frac{4}{n^3} \left[ \frac{n(n+1)(2n+1)}{6} \right] - \frac{5}{n^2} \left[ \frac{n(n+1)}{2} \right] + \frac{2}{n} \cdot n$$

$$\text{Area} = -\frac{1}{4} + \frac{4}{3} - \frac{5}{2} + 2 = \boxed{\frac{7}{12}}$$